GPUCSL/Lang.v
@@ -11,6 +11,7 @@ Require ClassicalFacts.
 Require Export FunctionalExtensionality.
 Require Export ProofIrrelevance.
 Require Import String.
+Require Import Sumbool.
 
 Require Export Coq.ZArith.BinInt.
 
@@ -25,8 +26,13 @@ Inductive PL := Shared | Global.
 Inductive loc := Loc (pl : PL) (l : Z).
 Notation SLoc := (Loc Shared).
 Notation GLoc := (Loc Global).
+
+Inductive val :=
+| VZ (n : Z)
+| VPtr (l : loc).
+
 Inductive var := Var : string -> var.
-Definition stack := var -> Z.
+Definition stack := var -> val.
 Require Import Classes.EquivDec.
 Global Program Instance loc_eq_dec : eq_type loc.
 Next Obligation.
@@ -37,39 +43,26 @@ Next Obligation.
   apply Z_eq_dec.
 Defined.
 
-Notation heap := (heap loc).
-Notation pheap' := (gen_pheap' loc).
-Notation pheap := (gen_pheap loc).
+Notation heap := (@heap loc val).
+Notation pheap' := (@gen_pheap' loc val).
+Notation pheap := (@gen_pheap loc val).
 Definition state := (stack * heap)%type.
 Arguments eq_dec _ _ _ _ : simpl never.
 
-Inductive binop_exp :=
-| OP_plus | OP_min | OP_lt | OP_eq | OP_mult | OP_sub | OP_div | OP_mod.
+Inductive binop :=
+| OP_plus | OP_min | OP_eq | OP_lt | OP_mult | OP_sub | OP_div | OP_mod (* Arith *)
+| OP_and | OP_or (* Boolean *).
+
+Inductive unop :=
+| OP_not.
 
 Inductive exp := 
 | Evar (x : var)
 | Enum (n : Z)
-| Ebinop (op : binop_exp) (e1 e2 : exp).
+| Eunop (op : unop) (e : exp)
+| Ebinop (op : binop) (e1 e2 : exp).
 
-Inductive binop_comp :=
-| OP_beq | OP_blt.
-
-Inductive binop_bool :=
-| OP_and | OP_or.
-
-Inductive unop_bool :=
-| OP_not.
-
-Inductive bexp :=
-| Bcomp (op : binop_comp) (e1 e2 : exp)
-| Bbool (op : binop_bool) (b1 b2 : bexp)
-| Bunary (op : unop_bool) (b : bexp).
-
-Inductive loc_exp :=
-| Addr : PL -> exp -> loc_exp
-| loc_offset : loc_exp -> exp -> loc_exp.
-Notation Sh := (Addr Shared).
-Notation Gl := (Addr Global).
+Inductive loc_exp := Loff (base off : exp).
 
 Inductive CTyp := Int | Bool | Ptr (cty : CTyp).
 
@@ -79,8 +72,8 @@ Inductive cmd : Set :=
 | Cread (typ : option CTyp) (x: var) (e: loc_exp)
 | Cwrite (e1: loc_exp) (e2: exp)
 | Cseq (c1: cmd) (c2: cmd)
-| Cif (b: bexp) (c1: cmd) (c2: cmd)
-| Cwhile (b: bexp) (c: cmd)
+| Cif (b: exp) (c1: cmd) (c2: cmd)
+| Cwhile (b: exp) (c: cmd)
 | Cbarrier (j : nat).
 
 Notation "'SKIP'" := Cskip.
@@ -106,57 +99,56 @@ Fixpoint wait (c : cmd) : option (nat * cmd) :=
       end
   end.
 
-Fixpoint binop_exp_denot op :=
+Definition binop_denote op x y :=
   match op with
-  | OP_plus => Z.add
-  | OP_min => Z.min
-  | OP_lt => fun x y => if Z_lt_dec x y then 1 else 0
-  | OP_eq => fun x y => if eq_dec x y then 1 else 0
-  | OP_mult => Z.mul
-  | OP_sub => Z.sub
-  | OP_div => Z.div
-  | OP_mod => Z.modulo
+  | OP_plus => Some (Z.add x y)
+  | OP_min => Some (Z.min x y)
+  | OP_lt => if Z_lt_dec x y then Some 1 else Some 0
+  | OP_eq => if eq_dec x y then Some 1 else Some 0
+  | OP_mult => Some (Z.mul x y)
+  | OP_sub => Some (Z.sub x y)
+  | OP_div => if eq_dec y 0 then None else Some (Z.div x y)
+  | OP_mod => if eq_dec y 0 then None else Some (Z.modulo x y)
+  | OP_and => if sumbool_or _ _ _ _ (eq_dec x 0) (eq_dec y 0) then Some 0 else Some 1
+  | OP_or => if sumbool_and _ _ _ _ (eq_dec x 0) (eq_dec y 0) then Some 0 else Some 1
   end%Z.
 
-Fixpoint edenot e s :=
-  match e with
-    | Evar v => s v
-    | Enum n => n
-    | Ebinop op e1 e2 => binop_exp_denot op (edenot e1 s) (edenot e2 s)
+Fixpoint unop_denote op x :=
+  match op with
+  | OP_not => if eq_dec x 0 then 1 else 0
   end%Z.
 
-Fixpoint ledenot e s :=
+Fixpoint edenote e (s : stack) : option val :=
   match e with
-    | Addr p e => Loc p (edenot e s)
-    | loc_offset e e' =>
-      match ledenot e s with
-      | Loc p lv => Loc p (lv + edenot e' s)
+    | Evar v => Some (s v)
+    | Enum n => Some (VZ n)
+    | Eunop op e =>
+      match edenote e s with
+      | Some (VZ v) => Some (VZ (unop_denote op v))
+      | _ => None
+      end
+    | Ebinop op e1 e2 =>
+      match edenote e1 s, edenote e2 s with
+      | Some (VZ v1), Some (VZ v2) =>
+        match binop_denote op v1 v2 with
+        | Some v => Some (VZ v)
+        | None => None
+        end
+      | _, _ =>
+        None
       end
   end%Z.
 
-Fixpoint binop_comp_denot op :=
-  match op with 
-  | OP_beq => fun x y => if eq_dec x y then true else false
-  | OP_blt => fun x y => if Z_lt_dec x y then true else false
-  end.
+Fixpoint ledenote e s :=
+  match e with
+  | Loff base off =>
+    match edenote base s, edenote off s with
+    | Some (VPtr (Loc pl p)), Some (VZ o) => 
+      Some (Loc pl (p + o))
+    | _, _ => None
+    end
+  end%Z.
 
-Fixpoint binop_bool_denot op :=
-  match op with
-  | OP_and => andb
-  | OP_or => orb
-  end.
-
-Fixpoint unop_bool_denot op :=
-  match op with
-  | OP_not => negb
-  end.
-
-Fixpoint bdenot b s : bool := 
-  match b with
-  | Bcomp op e1 e2 => binop_comp_denot op (edenot e1 s) (edenot e2 s)
-  | Bbool op b1 b2 => binop_bool_denot op (bdenot b1 s) (bdenot b2 s)
-  | Bunary op b => unop_bool_denot op (bdenot b s)
-  end.
 
 Lemma var_eq_dec (x y : var) : {x = y} + {x <> y}.
 Proof.
@@ -171,26 +163,31 @@ Inductive red: cmd -> state -> cmd  -> state -> Prop :=
 | red_Seq2: forall (c1 : cmd) (ss : state) (c1' : cmd) (ss' : state) (c2 : cmd)
                    (R: c1 / ss ==>s c1' / ss'), 
               (c1 ;; c2) / ss ==>s (c1' ;; c2) / ss'
-| red_If1: forall (b : bexp) (c1 c2 : cmd) (ss : state) 
-                  (B: bdenot b (fst ss) = true), 
+| red_If1: forall (b : exp) (v : Z) (c1 c2 : cmd) (ss : state) 
+                  (B: edenote b (fst ss) = Some (VZ v))
+                  (Bt: v <> 0%Z),
              (Cif b c1 c2) / ss ==>s c1 / ss
-| red_If2: forall (b : bexp) (c1 c2 : cmd) (ss : state)
-                  (B: bdenot b (fst ss) = false),
+| red_If2: forall (b : exp) (c1 c2 : cmd) (ss : state)
+                  (B: edenote b (fst ss) = Some (VZ 0%Z)),
              (Cif b c1 c2) / ss ==>s c2 / ss
-| red_Loop: forall (b : bexp) (c : cmd) (ss : state),  
+| red_Loop: forall (b : exp) (c : cmd) (ss : state),  
              (Cwhile b c) / ss ==>s (Cif b (Cseq c (Cwhile b c)) Cskip) / ss
-| red_Assign: forall (x : var) (e : exp) (cty : option CTyp) ss ss' s h
+| red_Assign: forall (x : var) (e : exp) (v : val) (cty : option CTyp) ss ss' s h
                      (EQ1: ss = (s, h))
-                     (EQ2: ss' = (var_upd s x (edenot e s), h)),
+                     (Eval: edenote e s = Some v)
+                     (EQ2: ss' = (var_upd s x v, h)),
                 (x ::T cty ::= e) / ss ==>s Cskip / ss'
-| red_Read: forall x e ss ss' (cty : option CTyp) s h v
+| red_Read: forall x e l ss ss' (cty : option CTyp) s h v
                    (EQ1: ss = (s, h))
-                   (RD: h (ledenot e s) = Some v)
+                   (Eval: ledenote e s = Some l)
+                   (RD: h l = Some v)
                    (EQ2: ss' = (var_upd s x v, h)),
               (x ::T cty ::= [e]) / ss ==>s Cskip / ss'
-| red_Write: forall e1 e2 ss ss' s h
+| red_Write: forall e1 e2 l v ss ss' s h
                     (EQ1: ss = (s, h))
-                    (EQ2: ss' = (s, upd h (ledenot e1 s) (Some (edenot e2 s)))),
+                    (Eval1: ledenote e1 s = Some l)
+                    (Eval2: edenote e2 s = Some v)
+                    (EQ2: ss' = (s, upd h l (Some v))),
                (Cwrite e1 e2) / ss ==>s Cskip / ss'
                               where  "c '/' st  '==>s'  c' '/' st' " := (red c st c' st').
 
@@ -219,8 +216,8 @@ Fixpoint accesses (c : cmd) (s : stack) :=
   match c with
     | Cskip => None
     | x ::T _ ::= e => None
-    | x ::T _ ::= [e] => Some (ledenot e s)
-    | [e] ::= e' => Some (ledenot e s)
+    | x ::T _ ::= [e] => ledenote e s
+    | [e] ::= e' => ledenote e s
     | c1 ;; c2 => accesses c1 s
     | (Cif b c1 c2) => None
     | (Cwhile b c) => None
@@ -232,7 +229,7 @@ Fixpoint writes (c : cmd) (s : stack) :=
     | Cskip => None
     | (x ::T _ ::= e) => None
     | (x ::T _ ::= [e]) => None
-    | ([e] ::= e') => Some (ledenot e s)
+    | ([e] ::= e') => ledenote e s
     | (c1 ;; c2) => writes c1 s
     | (Cif b c1 c2) => None
     | (Cwhile b c) => None
@@ -241,12 +238,26 @@ Fixpoint writes (c : cmd) (s : stack) :=
 
 Inductive aborts : cmd -> state -> Prop := 
 | aborts_Seq : forall (c1 c2 : cmd) (ss : state) (A: aborts c1 ss), aborts (Cseq c1 c2) ss
-| aborts_Read: forall x e ty ss
-                      (NIN: snd ss (ledenot e (fst ss)) = None),
-                 aborts (Cread x ty e) ss
-| aborts_Write: forall e1 e2 ss
-                       (NIN: snd ss (ledenot e1 (fst ss)) = None),
-                  aborts (Cwrite e1 e2) ss.
+| aborts_Assign : forall x ty e ss
+                         (EVAL: edenote e (fst ss) = None),
+    aborts (Cassign ty x e) ss
+| aborts_Read1: forall x e ty ss
+                       (EVAL: ledenote e (fst ss) = None),
+    aborts (Cread ty x e) ss
+| aborts_Read2: forall x e l ty ss
+                       (EVAL: ledenote e (fst ss) = Some l)
+                       (NIN: snd ss l = None),
+    aborts (Cread x ty e) ss
+| aborts_Write1: forall e1 e2 ss
+                       (EVAL: ledenote e1 (fst ss) = None),
+    aborts (Cwrite e1 e2) ss
+| aborts_Write2: forall e1 e2 l ss
+                        (EVAL: ledenote e1 (fst ss) = Some l)
+                        (NIN: snd ss l = None),
+    aborts (Cwrite e1 e2) ss
+| aborts_If: forall e c1 c2 ss
+                      (Eval: edenote e (fst ss) = None),
+    aborts (Cif e c1 c2) ss.
 
 Fixpoint barriers c :=
   match c with
@@ -260,44 +271,44 @@ Fixpoint barriers c :=
     | Cbarrier j => j :: nil
   end.
 
-Lemma naborts_red_s (c1 c2 : cmd) (s1 s2 : stack) (h1 h2 hF : heap) :
-  hdisj h1 hF -> hdisj h2 hF ->
-  ~aborts c1 (s1, h1) ->
-  c1 / (s1, hplus h1 hF) ==>s c2 / (s2, hplus h2 hF) ->
-  c1 / (s1, h1) ==>s c2 / (s2, h2).
-Proof.
-  intros hdis1 hdis2 naborts hred.
-  remember (s1, hplus h1 hF) as st1.
-  remember (s2, hplus h2 hF) as st2.
-  induction hred; try constructor; eauto;
-  try (destruct ss as [s h]; inversion Heqst1; inversion Heqst2;
-       assert (h1 = h2) by (apply (hplus_cancel_l hdis1 hdis2 H1); eauto);
-       repeat subst; constructor; eauto).
-  - apply IHhred; eauto.
-    intros H; apply naborts; constructor; eauto.
-  - econstructor; eauto.
-    destruct ss, ss'. 
-    repeat match goal with | [ H : (_, _) = (_, _) |- _ ] => inversion H; clear H end; subst.
-    rewrite <-H4, H6.
-    cutrewrite (h1 = h2); [eauto | apply (hplus_cancel_l (h := h) hdis1 hdis2); eauto].
-  - apply (@red_Read _ _ _ _ _ s1 h1 v); eauto;
-    destruct ss as [s1' h1F], ss' as [s2' h2F];
-    repeat match goal with  | [ H : (_, _) = (_, _) |- _ ] => inversion H; clear H end; subst.
-    + rewrite H7 in RD.
-      destruct (hplus_map hdis1 RD) as [[? ?]| [? ?]]; [congruence|].
-      contradict naborts; constructor; subst; eauto.
-    + cut (h2 = h1 /\ s2 = var_upd s1 x v); [intros [? ?]; rewrite <-H4; subst; eauto|].
-      split; [eapply (hplus_cancel_l hdis2); eauto | congruence].
-  - apply (@red_Write _ _ _ _ s1 h1); eauto.
-    destruct ss as [sx hx], ss' as [sx' hx'].
-    repeat match goal with | [ H : (_, _) = (_, _) |- _ ] => inversion H; clear H end; subst.
-    cut (s2 = s1 /\ h2 = upd h1 (ledenot e1 s1) (Some (edenot e2 s1))); 
-      [intros [? ?]; subst; eauto|].
-    split; [congruence|].
-    rewrite <-H6; rewrite H7 in H5.
-    destruct (hplus_upd hdis1 hdis2 H5) as [? | [hFx ?]]; eauto.
-    contradict naborts; constructor; simpl; destruct (hdis1 (ledenot e1 s1)); congruence.
-Qed.
+(* Lemma naborts_red_s (c1 c2 : cmd) (s1 s2 : stack) (h1 h2 hF : heap) : *)
+(*   hdisj h1 hF -> hdisj h2 hF -> *)
+(*   ~aborts c1 (s1, h1) -> *)
+(*   c1 / (s1, hplus h1 hF) ==>s c2 / (s2, hplus h2 hF) -> *)
+(*   c1 / (s1, h1) ==>s c2 / (s2, h2). *)
+(* Proof. *)
+(*   intros hdis1 hdis2 naborts hred. *)
+(*   remember (s1, hplus h1 hF) as st1. *)
+(*   remember (s2, hplus h2 hF) as st2. *)
+(*   induction hred; try constructor; eauto; *)
+(*   try (destruct ss as [s h]; inversion Heqst1; inversion Heqst2; *)
+(*        assert (h1 = h2) by (apply (hplus_cancel_l hdis1 hdis2 H1); eauto); *)
+(*        repeat subst; constructor; eauto). *)
+(*   - apply IHhred; eauto. *)
+(*     intros H; apply naborts; constructor; eauto. *)
+(*   - econstructor; eauto. *)
+(*     destruct ss, ss'.  *)
+(*     repeat match goal with | [ H : (_, _) = (_, _) |- _ ] => inversion H; clear H end; subst. *)
+(*     rewrite <-H4, H6. *)
+(*     cutrewrite (h1 = h2); [eauto | apply (hplus_cancel_l (h := h) hdis1 hdis2); eauto]. *)
+(*   - apply (@red_Read _ _ _ _ _ s1 h1 v); eauto; *)
+(*     destruct ss as [s1' h1F], ss' as [s2' h2F]; *)
+(*     repeat match goal with  | [ H : (_, _) = (_, _) |- _ ] => inversion H; clear H end; subst. *)
+(*     + rewrite H7 in RD. *)
+(*       destruct (hplus_map hdis1 RD) as [[? ?]| [? ?]]; [congruence|]. *)
+(*       contradict naborts; constructor; subst; eauto. *)
+(*     + cut (h2 = h1 /\ s2 = var_upd s1 x v); [intros [? ?]; rewrite <-H4; subst; eauto|]. *)
+(*       split; [eapply (hplus_cancel_l hdis2); eauto | congruence]. *)
+(*   - apply (@red_Write _ _ _ _ s1 h1); eauto. *)
+(*     destruct ss as [sx hx], ss' as [sx' hx']. *)
+(*     repeat match goal with | [ H : (_, _) = (_, _) |- _ ] => inversion H; clear H end; subst. *)
+(*     cut (s2 = s1 /\ h2 = upd h1 (ledenot e1 s1) (Some (edenot e2 s1)));  *)
+(*       [intros [? ?]; subst; eauto|]. *)
+(*     split; [congruence|]. *)
+(*     rewrite <-H6; rewrite H7 in H5. *)
+(*     destruct (hplus_upd hdis1 hdis2 H5) as [? | [hFx ?]]; eauto. *)
+(*     contradict naborts; constructor; simpl; destruct (hdis1 (ledenot e1 s1)); congruence. *)
+(* Qed. *)
 
 Fixpoint disjoint_list A (l : list A) :=
   match l with
@@ -364,7 +375,7 @@ Module PLang.
     eapply padd_cancel2; eauto.
   Qed.
 
-  Lemma padd_upd_cancel (ph1 ph2 phF : pheap) (h : heap) (x : loc) (v v' : Z) :
+  Lemma padd_upd_cancel (ph1 ph2 phF : pheap) (h : heap) (x : loc) (v v' : val) :
     pdisj ph1 phF -> pdisj ph2 phF -> ptoheap (phplus ph1 phF) h ->
     this ph1 x = Some (full_p, v') -> ptoheap (phplus ph2 phF) (upd h x (Some v)) -> 
     this ph2 = ph_upd ph1 x v.
@@ -399,90 +410,90 @@ Module PLang.
       ring_simplify in H4; rewrite H4 in H; inversion H.
   Qed.
 
-  Lemma red_p_det (c c1 c2 : cmd) (st st1 st2 : pstate) :
-    c / st ==>p c1 / st1 ->
-    c / st ==>p c2 / st2 ->
-    c1 = c2 /\ st1 = st2.
-  Proof.
-    intros red1 red2.
-    destruct red1 as
-        [c1 c1' st1 st1' pst1 pst1' s1 s1' ph1 ph1' phF1 h1 h1' eq1 eq1' 
-            peq1 peq1' aok1 wok1 dis1 to1 red1 dis1' to1'].
-    destruct red2 as
-        [c2 c2' st2 st2' pst2 pst2' s2 s2' ph2 ph2' phF2 h2 h2' eq2 eq2' 
-            peq2 peq2' aok2 wok2 dis2 to2 red2 dis2' to2'].
-    revert c2' red2; induction red1; intros c2' red2; 
-    try (inversion red2; subst; 
-         repeat (match goal with [H : (_, _) = (_, _) |- _ ] => inversion H; subst; clear H end);
-         simpl in *; try congruence;
-         assert (ph1' = ph2) by (eapply phplus_cancel_toheap; eauto);
-         assert (ph2' = ph2) by (eapply phplus_cancel_toheap; eauto);
-         split; congruence).
-    - inversion red2; subst.
-      + repeat (match goal with [H : (_, _) = (_, _) |- _ ] => inversion H; subst; clear H end).
-        assert (ph1' = ph2) by (eapply phplus_cancel_toheap; eauto).
-        assert (ph2' = ph2) by (eapply phplus_cancel_toheap; eauto).
-        split; congruence.
-      + inversion R.
-    - inversion red2; subst. 
-      + inversion red1.
-      + unfold access_ok, write_ok in *; simpl in *. 
-        pose proof (IHred1 eq_refl eq_refl aok1 wok1 aok2 wok2 c1'0 R) as H; 
-          destruct H as [He1 He2].
-        split; [subst; eauto | eauto].
-    - inversion red2; subst;
-      repeat (match goal with [H : (_, _) = (_, _) |- _ ] => inversion H; subst; clear H end).
-      unfold access_ok in *; simpl in *.
-      remember (ledenot e s0) as vad.
-      assert (ph1' = ph2) by (eapply phplus_cancel_toheap; eauto).
-      assert (ph2' = ph2) by (eapply phplus_cancel_toheap; eauto).
-      cutrewrite (v = v0); [split; congruence |].
-      assert (Some v0 = Some v) as Heq; [ rewrite <- RD0, <-RD | 
-                                          rewrite <-RD0, <-RD in Heq; congruence].
-      clear Heqvad; subst.
-      destruct aok1 as [[q va] Hv].
-      unfold pdisj, ptoheap in *.
-      repeat (match goal with [H : forall _ : loc, _ |- _] => specialize (H vad) end).
-      unfold phplus in *.
-      rewrite Hv in *.
-      destruct (this phF1 vad) as [[? ?] | ], (this phF2 vad) as [[? ?] | ]; intuition; try congruence.
-    - inversion red2; subst.
-      split; eauto.
-      assert (s1' = s2') by congruence; subst.
-      assert (ph1' = ph2'); [| subst; eauto].
-      inversion EQ3; inversion EQ0; inversion peq2; inversion EQ2; inversion EQ1. 
-      subst. rewrite H8 in *.
-      unfold write_ok in *; simpl in *.
-      destruct wok1 as [v1' H1], wok2 as [v2' H2].
-      remember (ledenot e1 s) as addr. clear Heqaddr.
-      remember (edenot e2 s) as v. clear Heqv.
-      assert (this ph1' = ph_upd ph2 addr v) by eapply (padd_upd_cancel dis1 dis1' to1 H1 to1').
-      assert (this ph2' = ph_upd ph2 addr v) by eapply (padd_upd_cancel dis2 dis2' to2 H2 to2').
-      destruct ph1' as [ph1' h1], ph2' as [ph2' h2]; simpl in *; subst.
-      assert (h1 = h2) by apply proof_irrelevance; congruence.
-  Qed.
+  (* Lemma red_p_det (c c1 c2 : cmd) (st st1 st2 : pstate) : *)
+  (*   c / st ==>p c1 / st1 -> *)
+  (*   c / st ==>p c2 / st2 -> *)
+  (*   c1 = c2 /\ st1 = st2. *)
+  (* Proof. *)
+  (*   intros red1 red2. *)
+  (*   destruct red1 as *)
+  (*       [c1 c1' st1 st1' pst1 pst1' s1 s1' ph1 ph1' phF1 h1 h1' eq1 eq1'  *)
+  (*           peq1 peq1' aok1 wok1 dis1 to1 red1 dis1' to1']. *)
+  (*   destruct red2 as *)
+  (*       [c2 c2' st2 st2' pst2 pst2' s2 s2' ph2 ph2' phF2 h2 h2' eq2 eq2'  *)
+  (*           peq2 peq2' aok2 wok2 dis2 to2 red2 dis2' to2']. *)
+  (*   revert c2' red2; induction red1; intros c2' red2;  *)
+  (*   try (inversion red2; subst;  *)
+  (*        repeat (match goal with [H : (_, _) = (_, _) |- _ ] => inversion H; subst; clear H end); *)
+  (*        simpl in *; try congruence; *)
+  (*        assert (ph1' = ph2) by (eapply phplus_cancel_toheap; eauto); *)
+  (*        assert (ph2' = ph2) by (eapply phplus_cancel_toheap; eauto); *)
+  (*        split; congruence). *)
+  (*   - inversion red2; subst. *)
+  (*     + repeat (match goal with [H : (_, _) = (_, _) |- _ ] => inversion H; subst; clear H end). *)
+  (*       assert (ph1' = ph2) by (eapply phplus_cancel_toheap; eauto). *)
+  (*       assert (ph2' = ph2) by (eapply phplus_cancel_toheap; eauto). *)
+  (*       split; congruence. *)
+  (*     + inversion R. *)
+  (*   - inversion red2; subst.  *)
+  (*     + inversion red1. *)
+  (*     + unfold access_ok, write_ok in *; simpl in *.  *)
+  (*       pose proof (IHred1 eq_refl eq_refl aok1 wok1 aok2 wok2 c1'0 R) as H;  *)
+  (*         destruct H as [He1 He2]. *)
+  (*       split; [subst; eauto | eauto]. *)
+  (*   - inversion red2; subst; *)
+  (*     repeat (match goal with [H : (_, _) = (_, _) |- _ ] => inversion H; subst; clear H end). *)
+  (*     unfold access_ok in *; simpl in *. *)
+  (*     remember (ledenot e s0) as vad. *)
+  (*     assert (ph1' = ph2) by (eapply phplus_cancel_toheap; eauto). *)
+  (*     assert (ph2' = ph2) by (eapply phplus_cancel_toheap; eauto). *)
+  (*     cutrewrite (v = v0); [split; congruence |]. *)
+  (*     assert (Some v0 = Some v) as Heq; [ rewrite <- RD0, <-RD |  *)
+  (*                                         rewrite <-RD0, <-RD in Heq; congruence]. *)
+  (*     clear Heqvad; subst. *)
+  (*     destruct aok1 as [[q va] Hv]. *)
+  (*     unfold pdisj, ptoheap in *. *)
+  (*     repeat (match goal with [H : forall _ : loc, _ |- _] => specialize (H vad) end). *)
+  (*     unfold phplus in *. *)
+  (*     rewrite Hv in *. *)
+  (*     destruct (this phF1 vad) as [[? ?] | ], (this phF2 vad) as [[? ?] | ]; intuition; try congruence. *)
+  (*   - inversion red2; subst. *)
+  (*     split; eauto. *)
+  (*     assert (s1' = s2') by congruence; subst. *)
+  (*     assert (ph1' = ph2'); [| subst; eauto]. *)
+  (*     inversion EQ3; inversion EQ0; inversion peq2; inversion EQ2; inversion EQ1.  *)
+  (*     subst. rewrite H8 in *. *)
+  (*     unfold write_ok in *; simpl in *. *)
+  (*     destruct wok1 as [v1' H1], wok2 as [v2' H2]. *)
+  (*     remember (ledenot e1 s) as addr. clear Heqaddr. *)
+  (*     remember (edenot e2 s) as v. clear Heqv. *)
+  (*     assert (this ph1' = ph_upd ph2 addr v) by eapply (padd_upd_cancel dis1 dis1' to1 H1 to1'). *)
+  (*     assert (this ph2' = ph_upd ph2 addr v) by eapply (padd_upd_cancel dis2 dis2' to2 H2 to2'). *)
+  (*     destruct ph1' as [ph1' h1], ph2' as [ph2' h2]; simpl in *; subst. *)
+  (*     assert (h1 = h2) by apply proof_irrelevance; congruence. *)
+  (* Qed. *)
 
-  Lemma red_p_frame (c1 c2 : cmd) (pst1 pst2 : pstate) (hF : pheap) :
-    c1 / pst1 ==>p c2 / pst2 ->
-    pdisj hF (snd pst1) -> pdisj hF (snd pst2).
-  Proof.
-    intros hred; revert hF; case hred.
-    clear c1 c2 pst1 pst2 hred; 
-    intros c1 c2 st1 st2 pst1 pst2 s1 s2 ph1 ph2 phF h1 h2 hst1 hst2 hpst1 hpst2 haok hwok 
-           hdis1 htoh1 hred_s hdis2 htoh2 hF hdisF.
-    induction hred_s; subst;
-    try (inversion hst2; subst; rewrite<- (phplus_cancel_toheap hdis1 hdis2 htoh1 htoh2); tauto);
-    unfold access_ok, write_ok in *; simpl in *.
-    - apply IHhred_s; eauto.
-    - inversion EQ1; inversion EQ2; subst;
-      rewrite<- (phplus_cancel_toheap hdis1 hdis2 htoh1 htoh2); tauto.
-    - inversion EQ1; inversion EQ2; subst;
-      rewrite<- (phplus_cancel_toheap hdis1 hdis2 htoh1 htoh2); tauto.
-    - inversion EQ1; inversion EQ2; clear EQ1 EQ2; subst.
-      destruct hwok as [v' H].
-      rewrite (padd_upd_cancel hdis1 hdis2 htoh1 H htoh2).
-      apply pdisjC. rewrite pdisj_upd; eauto.
-  Qed.
+  (* Lemma red_p_frame (c1 c2 : cmd) (pst1 pst2 : pstate) (hF : pheap) : *)
+  (*   c1 / pst1 ==>p c2 / pst2 -> *)
+  (*   pdisj hF (snd pst1) -> pdisj hF (snd pst2). *)
+  (* Proof. *)
+  (*   intros hred; revert hF; case hred. *)
+  (*   clear c1 c2 pst1 pst2 hred;  *)
+  (*   intros c1 c2 st1 st2 pst1 pst2 s1 s2 ph1 ph2 phF h1 h2 hst1 hst2 hpst1 hpst2 haok hwok  *)
+  (*          hdis1 htoh1 hred_s hdis2 htoh2 hF hdisF. *)
+  (*   induction hred_s; subst; *)
+  (*   try (inversion hst2; subst; rewrite<- (phplus_cancel_toheap hdis1 hdis2 htoh1 htoh2); tauto); *)
+  (*   unfold access_ok, write_ok in *; simpl in *. *)
+  (*   - apply IHhred_s; eauto. *)
+  (*   - inversion EQ1; inversion EQ2; subst; *)
+  (*     rewrite<- (phplus_cancel_toheap hdis1 hdis2 htoh1 htoh2); tauto. *)
+  (*   - inversion EQ1; inversion EQ2; subst; *)
+  (*     rewrite<- (phplus_cancel_toheap hdis1 hdis2 htoh1 htoh2); tauto. *)
+  (*   - inversion EQ1; inversion EQ2; clear EQ1 EQ2; subst. *)
+  (*     destruct hwok as [v' H]. *)
+  (*     rewrite (padd_upd_cancel hdis1 hdis2 htoh1 H htoh2). *)
+  (*     apply pdisjC. rewrite pdisj_upd; eauto. *)
+  (* Qed. *)
 
   Lemma red_s_safe' (c1 c2 : cmd) (st1 st2 : state) (pst1 : pstate) (hF : pheap) :
     c1 / st1 ==>s c2 / st2 -> 
@@ -496,21 +507,21 @@ Module PLang.
     intros red1; revert pst1 hF; induction red1; intros pst1 hF hst hdis1 hto1 haok hwok;
     try (exists (snd pst1); subst; simpl; try destruct ss; split; tauto).
     - eapply IHred1; eauto.
-    - subst; rewrite hst in *; unfold access_ok, write_ok in *; simpl in *.
+    - subst; unfold access_ok, write_ok in *; simpl in *; rewrite hst, Eval1 in *.
       destruct hwok as [v' Hv'].
-      exists (Pheap (ph_upd_ph (snd pst1) (ledenot e1 s) (edenot e2 s))); simpl; split.
+      exists (Pheap (ph_upd_ph (snd pst1) l v)); simpl; split.
       + rewrite pdisj_upd; eauto.
-      + assert (this hF (ledenot e1 s) = None).
+      + assert (this hF l = None).
         { destruct hF as [hF isphF]; 
-          pose proof (hdis1 (ledenot e1 s)); pose proof (isphF (ledenot e1 s)); simpl in *.
-          rewrite Hv' in H. destruct (hF (ledenot e1 s)); eauto.
+          pose proof (hdis1 l); pose proof (isphF l); simpl in *.
+          rewrite Hv' in H. destruct (hF l); eauto.
           destruct p. destruct H0 as [H1 _], H as [_ [_ H2]].
           apply frac_contra1 in H2; eauto; tauto. } 
         intros x; unfold phplus, ph_upd, upd. 
-        specialize (hto1 x); destruct (eq_dec (ledenot e1 s) x).
+        specialize (hto1 x); destruct (eq_dec l x).
         * rewrite e, H in *; repeat split; unfold upd; destruct (eq_dec x x); try tauto.
         * unfold phplus,upd in *; destruct (this (snd pst1) x) as [[? ?]|], (this hF x) as [[? ?]|];
-          destruct (eq_dec x (ledenot e1 s)); 
+          destruct (eq_dec x l); 
           repeat split; try tauto; try congruence.
   Qed.
 
@@ -546,26 +557,32 @@ Module BigStep.
                   (c1 ;; c2) / st || Some (j, c1' ;; c2) / st'
   | eval_Seq2 : forall (c1 c2 : cmd) (c2' : option (nat * cmd)) (st st' st'' : pstate), 
                   c1 / st || None / st' -> c2 / st' || c2' / st'' -> (c1 ;; c2) / st || c2' / st''
-  | eval_If1 : forall (b : bexp) (c1 c2 : cmd) (c1' : option (nat * cmd)) (st st' : pstate),
-                 bdenot b (fst st) = true -> c1 / st || c1' / st' ->
+  | eval_If1 : forall (b : exp) v (c1 c2 : cmd) (c1' : option (nat * cmd)) (st st' : pstate),
+                 edenote b (fst st) = Some (VZ v) -> v <> 0%Z -> c1 / st || c1' / st' ->
                  (Cif b c1 c2) / st || c1' / st'
-  | eval_If2 : forall (b : bexp) (c1 c2 : cmd) (c2' : option (nat * cmd)) (st st' : pstate),
-                 bdenot b (fst st) = false -> c2 / st || c2' / st' ->
+  | eval_If2 : forall (b : exp) (c1 c2 : cmd) (c2' : option (nat * cmd)) (st st' : pstate),
+                 edenote b (fst st) = Some (VZ 0) -> c2 / st || c2' / st' ->
                  (Cif b c1 c2) / st || c2' / st'
-  | eval_Loop : forall (b : bexp) (c : cmd) (c' : option (nat * cmd)) (st st' : pstate),
+  | eval_Loop : forall (b : exp) (c : cmd) (c' : option (nat * cmd)) (st st' : pstate),
                   (Cif b (c ;; (Cwhile b c)) Cskip) / st || c'/ st' ->
                   (Cwhile b c) / st || c' / st'
-  | eval_Assign : forall (x : var) (e : exp) (cty : option CTyp) (st st' : pstate) s h,
-                    (st = (s, h)) -> (st' = (var_upd s x (edenot e s), h)) ->
+  | eval_Assign : forall (x : var) (e : exp) (v : val) (cty : option CTyp) (st st' : pstate) s h,
+                    (st = (s, h)) -> 
+                    (edenote e s = Some v) ->
+                    (st' = (var_upd s x v, h)) ->
                     (x ::T cty ::= e) / st || None / st'
-  | eval_Read : forall (x : var) (e : loc_exp) (cty : option CTyp) (v : Z) (st st' : pstate) (s : stack) (h : pheap) (q : Qc),
-                  (st = (s, h)) -> (this h (ledenot e s) = Some (q, v)) ->
+  | eval_Read : forall (x : var) (e : loc_exp) (l : loc) (cty : option CTyp) (v : val) (st st' : pstate) (s : stack) (h : pheap) (q : Qc),
+                  (st = (s, h)) -> 
+                  (ledenote e s = Some l) ->
+                  (this h l = Some (q, v)) ->
                   (st' = (var_upd s x v, h)) ->
                   (x ::T cty ::= [e]) / st || None / st'
-  | eval_Write : forall (e1 : loc_exp) (e2 : exp) (ss ss' : pstate) (s : stack) (h : pheap) (v : Z),
+  | eval_Write : forall (e1 : loc_exp) (e2 : exp) (ss ss' : pstate) (s : stack) (h : pheap) (l : loc) (v v' : val),
                    (ss = (s, h)) ->
-                   this h (ledenot e1 s) = Some (1, v) ->
-                   (ss' = (s, ph_upd2 h (ledenot e1 s) (edenot e2 s))) ->
+                   (ledenote e1 s = Some l) ->
+                   (edenote e2 s = Some v) ->
+                   this h l = Some (1, v') ->
+                   (ss' = (s, ph_upd2 h l v)) ->
                    (Cwrite e1 e2) / ss || None / ss'
   | eval_Barrier : forall ss j,
                      (Cbarrier j) / ss || Some (j, Cskip) / ss
@@ -586,25 +603,25 @@ Module BigStep.
     - inversion IH; subst; unfold access_ok, write_ok in *; simpl in *. 
       pose proof (IHred eq_refl eq_refl aok wok _ H1).
       econstructor; eauto.
-    (* - apply eval_If2; eauto. *)
+    - eapply eval_If1; eauto.
     - eapply eval_Assign; eauto.
       inversion IH; subst; eauto.
-    - unfold access_ok in *; simpl in *; destruct aok as [[q v'] h].
+    - unfold access_ok in *; simpl in *; rewrite Eval in *; destruct aok as [[q v'] h].
       eapply eval_Read; eauto.
       inversion IH; subst.
-      unfold ptoheap, phplus in to; specialize (to (ledenot e s0)); rewrite h in to;
-      destruct (this phF (ledenot e s0)) as [[? ?] |]; destruct to as [? H'];
+      unfold ptoheap, phplus in to; specialize (to l); rewrite h in to;
+      destruct (this phF l) as [[? ?] |]; destruct to as [? H'];
       rewrite H' in *; inversion RD; eauto.
-    - unfold write_ok in *; simpl in *; destruct wok as [v' h];
+    - unfold write_ok in *; simpl in *; rewrite Eval1 in *; destruct wok as [v' h];
       eapply eval_Write; eauto.
       inversion IH; subst; eauto.
-      cutrewrite (ph' = ph_upd2 ph (ledenot e1 s0) (edenot e2 s0)); eauto.
-      assert (this ph' = this (ph_upd2 ph (ledenot e1 s0) (edenot e2 s0))) by 
+      cutrewrite (ph' = ph_upd2 ph l v); eauto.
+      assert (this ph' = this (ph_upd2 ph l v)) by 
           (eapply padd_upd_cancel; eauto).
       destruct ph'; simpl in H.
       unfold ph_upd2.
       symmetry in H; destruct H.
-      cutrewrite (is_p = ph_upd_ph ph (ledenot e1 s0) (edenot e2 s0)); 
+      cutrewrite (is_p = ph_upd_ph ph l v); 
         [ eauto | apply proof_irrelevance ].
   Qed.
 
@@ -661,7 +678,7 @@ Module BigStep.
         * eapply eval_Seq2; eauto.
           eapply red1_eval; eauto.
           apply (@redp_ster _ _ (s, h) (s', h') (s, ph) (s', ph') s s' ph ph' phF h h'); eauto.
-      (* + apply eval_If2; eauto. *)
+      + eapply eval_If1; eauto.
       + inversion IH.
       + inversion IH.
       + inversion IH.
@@ -701,38 +718,38 @@ Notation "ks '==>k' ks'" := (red_k ks ks') (at level 40).
 Definition multi_red_k (ntrd : nat) (k1 k2 : kstate ntrd) := clos_refl_trans_1n _ (@red_k ntrd) k1 k2.
 Notation "ks '==>k*' ks'" := (multi_red_k ks ks') (at level 40).
 
-Section ParNAborts.
-  Variable ntrd : nat.
-  Import VectorNotations.
-  Lemma naborts_red_k (ks1 ks2 : klist ntrd) (h1 h2 hF : heap) :
-    hdisj h1 hF -> hdisj h2 hF ->
-    ~abort_k (ks1, h1) ->
-    (ks1, hplus h1 hF) ==>k (ks2, hplus h2 hF) ->
-    (ks1, h1) ==>k (ks2, h2).
-  Proof.
-    intros Hdis1 Hdis2 Hnaborts Hred.
-    remember (ks1, hplus h1 hF) as kss1; remember (ks2, hplus h2 hF) as kss2; 
-    destruct Hred.
-    - assert (~aborts c (s, h1)) as Hnab.
-      { intros Hc; contradict Hnaborts; exists i; simpl.
-        destruct ks; inversion Heqkss1; inversion H; repeat subst; destruct ss[@i]; inversion H0;
-        subst; eauto. }
-      rewrite H2, H3 in H1.
-      cutrewrite (h = hplus h1 hF) in H1; [|inversion Heqkss1; congruence].
-      cutrewrite (h' = hplus h2 hF) in H1; [|inversion Heqkss2; congruence].
-      apply naborts_red_s in H1; eauto.
-      inversion Heqkss2.
-      cutrewrite (ks1 = ss); [|destruct ks; inversion Heqkss1; inversion H; congruence].
-      apply (redk_Seq eq_refl H0 H1 eq_refl eq_refl).
-    - cutrewrite (ks1 = ss); [|destruct ks; inversion Heqkss1; inversion H; congruence].
-      cutrewrite (ks2 = ss'); [|destruct ks'; inversion Heqkss2; inversion H0; congruence].
-      assert (hplus h2 hF = hplus h1 hF) as H12eq.
-      { destruct ks, ks'; inversion Heqkss1; inversion Heqkss2; inversion H; inversion H0;
-        congruence. }
-      cutrewrite (h1 = h2); [| eapply (hplus_cancel_l (h := hplus h1 hF) Hdis1 Hdis2); congruence].
-      apply (redk_Barrier eq_refl eq_refl H1).
-  Qed.
-End ParNAborts.
+(* Section ParNAborts. *)
+(*   Variable ntrd : nat. *)
+(*   Import VectorNotations. *)
+(*   Lemma naborts_red_k (ks1 ks2 : klist ntrd) (h1 h2 hF : heap) : *)
+(*     hdisj h1 hF -> hdisj h2 hF -> *)
+(*     ~abort_k (ks1, h1) -> *)
+(*     (ks1, hplus h1 hF) ==>k (ks2, hplus h2 hF) -> *)
+(*     (ks1, h1) ==>k (ks2, h2). *)
+(*   Proof. *)
+(*     intros Hdis1 Hdis2 Hnaborts Hred. *)
+(*     remember (ks1, hplus h1 hF) as kss1; remember (ks2, hplus h2 hF) as kss2;  *)
+(*     destruct Hred. *)
+(*     - assert (~aborts c (s, h1)) as Hnab. *)
+(*       { intros Hc; contradict Hnaborts; exists i; simpl. *)
+(*         destruct ks; inversion Heqkss1; inversion H; repeat subst; destruct ss[@i]; inversion H0; *)
+(*         subst; eauto. } *)
+(*       rewrite H2, H3 in H1. *)
+(*       cutrewrite (h = hplus h1 hF) in H1; [|inversion Heqkss1; congruence]. *)
+(*       cutrewrite (h' = hplus h2 hF) in H1; [|inversion Heqkss2; congruence]. *)
+(*       apply naborts_red_s in H1; eauto. *)
+(*       inversion Heqkss2. *)
+(*       cutrewrite (ks1 = ss); [|destruct ks; inversion Heqkss1; inversion H; congruence]. *)
+(*       apply (redk_Seq eq_refl H0 H1 eq_refl eq_refl). *)
+(*     - cutrewrite (ks1 = ss); [|destruct ks; inversion Heqkss1; inversion H; congruence]. *)
+(*       cutrewrite (ks2 = ss'); [|destruct ks'; inversion Heqkss2; inversion H0; congruence]. *)
+(*       assert (hplus h2 hF = hplus h1 hF) as H12eq. *)
+(*       { destruct ks, ks'; inversion Heqkss1; inversion Heqkss2; inversion H; inversion H0; *)
+(*         congruence. } *)
+(*       cutrewrite (h1 = h2); [| eapply (hplus_cancel_l (h := hplus h1 hF) Hdis1 Hdis2); congruence]. *)
+(*       apply (redk_Barrier eq_refl eq_refl H1). *)
+(*   Qed. *)
+(* End ParNAborts. *)
   
 Section NonInter.
   Inductive type := Hi | Lo.
@@ -754,25 +771,16 @@ Section NonInter.
   Inductive typing_exp : exp -> type -> Prop := 
   | ty_var : forall (v : var) (ty : type), le_type (g v) ty = true -> typing_exp (Evar v) ty
   | ty_num : forall (n : Z) (ty : type), typing_exp (Enum n) ty
-  | ty_binop : forall (op : binop_exp) (e1 e2 : exp) (ty1 ty2 : type), 
+  | ty_unop : forall (op : unop) (e : exp) (ty : type), 
+                typing_exp e ty -> 
+                typing_exp (Eunop op e) ty
+  | ty_binop : forall (op : binop) (e1 e2 : exp) (ty1 ty2 : type), 
                 typing_exp e1 ty1 -> typing_exp e2 ty2 ->
                 typing_exp (Ebinop op e1 e2) (join ty1 ty2).
 
-  Inductive typing_bexp : bexp -> type -> Prop := 
-  | ty_comp : forall op (e1 e2 : exp) (ty1 ty2 : type),
-      typing_exp e1 ty1 -> typing_exp e2 ty2 ->
-      typing_bexp (Bcomp op e1 e2) (join ty1 ty2)
-  | ty_bool : forall op (e1 e2 : bexp) (ty1 ty2 : type),
-      typing_bexp e1 ty1 -> typing_bexp e2 ty2 ->
-      typing_bexp (Bbool op e1 e2) (join ty1 ty2)
-  | ty_unary : forall op (e : bexp) (ty : type),
-      typing_bexp e ty -> typing_bexp (Bunary op e) ty.
-
   Inductive typing_lexp : loc_exp -> type -> Prop :=
-  | ty_sloc : forall e ty, typing_exp e ty -> typing_lexp (Sh e) ty
-  | ty_gloc : forall e ty, typing_exp e ty -> typing_lexp (Gl e) ty
-  | ty_offset : forall e e' ty1 ty2, typing_lexp e ty1 -> typing_exp e' ty2 ->
-                                     typing_lexp (loc_offset e e') (join ty1 ty2).
+  | ty_off : forall e e' ty1 ty2, typing_exp e ty1 -> typing_exp e' ty2 ->
+                                  typing_lexp (Loff e e') (join ty1 ty2).
 
   Inductive typing_cmd : cmd -> type -> Prop :=
   | ty_skip : forall (pc : type), typing_cmd Cskip pc
@@ -787,18 +795,18 @@ Section NonInter.
   | ty_seq : forall (c1 c2 : cmd) (pc : type),
                typing_cmd c1 pc -> typing_cmd c2 pc ->
                typing_cmd (c1 ;; c2) pc
-  | ty_if : forall (b : bexp) (c1 c2 : cmd) (pc ty : type),
-              typing_bexp b ty ->
+  | ty_if : forall (b : exp) (c1 c2 : cmd) (pc ty : type),
+              typing_exp b ty ->
               typing_cmd c1 (join pc ty) -> typing_cmd c2 (join pc ty) ->
               typing_cmd (Cif b c1 c2) pc
-  | ty_while : forall (b : bexp) (c : cmd) (pc ty : type),
-                 typing_bexp b ty ->
+  | ty_while : forall (b : exp) (c : cmd) (pc ty : type),
+                 typing_exp b ty ->
                  typing_cmd c (join pc ty) -> typing_cmd (Cwhile b c) pc
   | ty_barrier : forall (j : nat), typing_cmd (Cbarrier j) Lo.
 
   Definition low_eq (s1 s2 : stack) := forall x, g x = Lo -> s1 x = s2 x.
   
-  Lemma hi_low_eq (x : var) (v1 v2 : Z) (s1 s2 : stack):
+  Lemma hi_low_eq (x : var) (v1 v2 : val) (s1 s2 : stack):
     low_eq s1 s2 -> g x = Hi -> low_eq (var_upd s1 x v1) (var_upd s2 x v2).
   Proof.
     unfold var_upd; intros heq hhi y; destruct (var_eq_dec y x); subst.
@@ -807,39 +815,29 @@ Section NonInter.
   Qed.
 
   Lemma low_eq_eq_exp (e : exp) (s1 s2 : stack) :
-    low_eq s1 s2 -> typing_exp e Lo -> edenot e s1 = edenot e s2.
+    low_eq s1 s2 -> typing_exp e Lo -> edenote e s1 = edenote e s2.
   Proof.
     intros heq hty; induction e; simpl; eauto; 
     try now (inversion hty; destruct ty1, ty2; unfold join in *; try congruence;
              rewrite IHe1, IHe2; eauto).
     - inversion hty; specialize (heq x).
-      destruct (g x); unfold le_type in H0; try congruence; eauto.
+      destruct (g x); unfold le_type in H0; try congruence.
+      rewrite heq; eauto.
+    - inversion hty. 
+      rewrite IHe; eauto.
   Qed.
 
   Lemma low_eq_eq_lexp (e : loc_exp) (s1 s2 : stack) :
-    low_eq s1 s2 -> typing_lexp e Lo -> ledenot e s1 = ledenot e s2.
+    low_eq s1 s2 -> typing_lexp e Lo -> ledenote e s1 = ledenote e s2.
   Proof.
-    intros; induction e; simpl; f_equal; inversion H0; auto using low_eq_eq_exp.
+    destruct e; intros; simpl.
+    inversion H0; subst.
     destruct ty1, ty2; inversion H3.
-    erewrite IHe, low_eq_eq_exp; eauto.
+    erewrite low_eq_eq_exp; eauto.
+    destruct edenote as [[? | [? ?]]|]; eauto.
+    erewrite low_eq_eq_exp; eauto.
   Qed.
   
-  Lemma low_eq_eq_bexp (be : bexp) (s1 s2 : stack) :
-    low_eq s1 s2 -> typing_bexp be Lo -> bdenot be s1 = bdenot be s2.
-  Proof.
-    intros heq hty; induction be; simpl; eauto.
-    - inversion hty; subst.
-      destruct ty1, ty2; inversion H3.
-      cutrewrite (edenot e1 s1 = edenot e1 s2); [ | eapply low_eq_eq_exp; eauto].
-      cutrewrite (edenot e2 s1 = edenot e2 s2); [ | eapply low_eq_eq_exp; eauto].
-      eauto.
-    - inversion hty.
-      destruct ty1, ty2; inversion H3.
-      rewrite IHbe1, IHbe2; eauto.
-    - inversion hty.
-      rewrite (IHbe H0); eauto.
-  Qed.
-
   Definition st_compat (st1 st2 : pstate) :=
     low_eq (fst st1) (fst st2) /\ pdisj (snd st1) (snd st2).
 
@@ -867,7 +865,7 @@ Section NonInter.
       eauto.
     - inversion htng1; subst.
       cutrewrite (join ty Hi = Hi) in H6; [ | destruct ty; eauto].
-      assert (g x = Hi) by (destruct (g x); inversion H6; eauto).
+      assert (g x = Hi) by (destruct (g x), ty; inversion H7; eauto).
       destruct hcomp as [heq ?];
         repeat split; destruct st1 as [s1 h1]; simpl; eauto.
       intros y; unfold var_upd; destruct (var_eq_dec y x); subst.
@@ -875,14 +873,14 @@ Section NonInter.
       + specialize (heq y); eauto.
     - inversion htng1; subst.
       cutrewrite (join ty Hi = Hi) in H7; [ | destruct ty; eauto].
-      assert (g x = Hi) by (destruct (g x); inversion H7; eauto).
+      assert (g x = Hi) by (destruct (g x), ty; inversion H8; eauto).
       destruct st1 as [s' h'], hcomp as [heq hdisj]; simpl in *.
       repeat split; eauto; simpl.
       intros y; unfold var_upd; destruct (var_eq_dec y x); subst.
       + intros H'; congruence.
       + specialize (heq y); simpl; eauto.
     - subst; destruct st1, hcomp; unfold st_compat in *; simpl in *; repeat split; eauto.
-      apply pdisjC. apply (pdisj_upd _ _ H0); apply pdisjC; eauto.
+      apply pdisjC. apply (pdisj_upd _ _ H2); apply pdisjC; eauto.
     - inversion htng1.
   Qed.
 
@@ -925,26 +923,26 @@ Section NonInter.
       + pose proof (IHev1_1 H1 _ _ _ hcomp H2) as [_ hcomp'].
         apply (IHev1_2 H3 _ _ _ hcomp' H7).
     - inversion htng; subst.
-      rename H3 into htngb, H5 into htng1, H6 into htng2.
+      rename H4 into htngb, H6 into htng1, H7 into htng2.
       inversion ev2; subst.
       + destruct ty0.
         * assert (join ty Hi = Hi) as Hr by (destruct ty; eauto); rewrite Hr in *; clear Hr.
-          eapply (non_interference_hi2 htng1 htng1 hcomp ev1 H7).
-        * destruct ty; [eapply (non_interference_hi2 htng1 htng1 hcomp ev1 H7)|].
+          eapply (non_interference_hi2 htng1 htng1 hcomp ev1 H9).
+        * destruct ty; [eapply (non_interference_hi2 htng1 htng1 hcomp ev1 H9)|].
           apply (IHev1 htng1 _ _ _ hcomp); eauto.
       + destruct ty0.
         * assert (join ty Hi = Hi) as Hr by (destruct ty; eauto); rewrite Hr in *; clear Hr.
-          eapply (non_interference_hi2 htng1 htng2 hcomp ev1 H7).
-        * destruct ty; [eapply (non_interference_hi2 htng1 htng2 hcomp ev1 H7)|].
-          pose proof (low_eq_eq_bexp (proj1 hcomp) htngb); congruence.
+          eapply (non_interference_hi2 htng1 htng2 hcomp ev1 H8).
+        * destruct ty; [eapply (non_interference_hi2 htng1 htng2 hcomp ev1 H8)|].
+          pose proof (low_eq_eq_exp (proj1 hcomp) htngb); congruence.
     - inversion htng; subst.
       rename H3 into htngb, H5 into htng1, H6 into htng2.
       inversion ev2; subst.
       + destruct ty0.
         * assert (join ty Hi = Hi) as Hr by (destruct ty; eauto); rewrite Hr in *; clear Hr.
-          eapply (non_interference_hi2 htng2 htng1  hcomp ev1 H7).
-        * destruct ty; [eapply (non_interference_hi2 htng2 htng1 hcomp ev1 H7)|].
-          pose proof (low_eq_eq_bexp (proj1 hcomp) htngb); congruence.
+          eapply (non_interference_hi2 htng2 htng1  hcomp ev1 H8).
+        * destruct ty; [eapply (non_interference_hi2 htng2 htng1 hcomp ev1 H8)|].
+          pose proof (low_eq_eq_exp (proj1 hcomp) htngb); congruence.
       + destruct ty0.
         * assert (join ty Hi = Hi) as Hr by (destruct ty; eauto); rewrite Hr in *; clear Hr.
           eapply (non_interference_hi2 htng2 htng2 hcomp ev1 H7).
@@ -959,35 +957,37 @@ Section NonInter.
       + inversion H7; subst.
         inversion ev1; subst; try (inversion H9; subst; tauto).
         destruct ty; inversion htng; subst.
-        * cutrewrite (join Hi ty = Hi) in H3; [|eauto].
+        * cutrewrite (join Hi ty = Hi) in H5; [|eauto].
           pose proof (st_compat_sym hcomp).
           assert (typing_cmd (c ;; Cwhile b c) Hi) by (econstructor; eauto).
-          pose proof (non_interference_hi H0 H H9).
-          destruct H2 as [? H']; split; [eauto | apply (st_compat_sym H')].
+          pose proof (non_interference_hi H0 H H10).
+          destruct H3 as [? H']; split; [eauto | apply (st_compat_sym H')].
         * destruct ty.
           { assert (typing_cmd (Cwhile b c) Hi) by (econstructor; eauto).
             assert (typing_cmd (c;; Cwhile b c) Hi) by (econstructor; eauto).
-            pose proof (non_interference_hi H0 (st_compat_sym hcomp) H9).
-            destruct H2 as [? H']; split; [eauto | apply (st_compat_sym H')]. }
-          pose proof (low_eq_eq_bexp (proj1 hcomp) H1); congruence.
+            pose proof (non_interference_hi H0 (st_compat_sym hcomp) H10).
+            destruct H3 as [? H']; split; [eauto | apply (st_compat_sym H')]. }
+          pose proof (low_eq_eq_exp (proj1 hcomp) H1); congruence.
     - inversion ev2; subst; simpl in *; repeat split; eauto; [|  intuition eauto].
       destruct ty; inversion htng; subst.
-      + inversion H4; apply hi_low_eq; intuition eauto.
-        destruct ty, (g x); unfold le_type in *; simpl in *; inversion H4; eauto.
+      + inversion H5; apply hi_low_eq; intuition eauto.
+        destruct ty, (g x); unfold le_type in *; simpl in *; inversion H5; eauto.
       + intros y hlo; pose proof ((proj1 hcomp) y hlo); unfold var_upd; destruct (var_eq_dec y x); eauto; subst.
-        eapply low_eq_eq_exp; intuition eauto.
-        destruct ty, (g x); simpl in H4; inversion H4; inversion hlo; eauto.
+        erewrite low_eq_eq_exp in H0; intuition eauto.
+        rewrite H0 in H9; inversion H9; eauto.
+        destruct ty, (g x); simpl in H5; inversion H5; inversion hlo; eauto.
     - inversion ev2; subst; simpl in *; repeat split; [ | intuition eauto].
       destruct ty; inversion htng; subst.
       + apply hi_low_eq; intuition eauto.
-        destruct ty, (g x); unfold le_type in *; simpl in *; inversion H5; intuition eauto.
+        destruct ty, (g x); unfold le_type in *; simpl in *; inversion H6; intuition eauto.
       + intros y hlo; pose proof ((proj1 hcomp) y hlo); unfold var_upd; destruct (var_eq_dec y x); eauto; subst.
-        destruct ty, (g x); simpl in H5; inversion H5; inversion hlo; eauto.
-        assert (ledenot e s = ledenot e s0) by (apply low_eq_eq_lexp; intuition eauto).
-        rewrite H1 in *.
+        destruct ty, (g x); simpl in H6; inversion H6; inversion hlo; eauto.
+        assert (ledenote e s = ledenote e s0) by (apply low_eq_eq_lexp; intuition eauto).
+        rewrite H2 in *.
+        rewrite H0 in H7; inversion H7; subst.
         eapply pheap_disj_eq; intuition eauto.
     - inversion ev2; subst; simpl in *; repeat split; intuition eauto.
-      apply (pheap_disj_disj _ _ H1 H0 H5).
+      apply (pheap_disj_disj _ _ H3 H2 H9).
     - inversion ev2; subst; repeat split; intuition eauto.
   Qed.
 
@@ -1062,58 +1062,53 @@ Section NonInter.
   Qed.
 End NonInter.
 
-Section Substitution.
-  (* from CSLsound.v *)
-  Fixpoint subE x e e0 := 
-    match e0 with 
-      | Evar y => (if var_eq_dec x y then e else Evar y)
-      | Enum n => Enum n
-      | Ebinop op e1 e2 => Ebinop op (subE x e e1) (subE x e e2)
-    end.
-  Fixpoint sublE x e e0 := 
-    match e0 with 
-      | Sh e0 => Sh (subE x e e0)
-      | Gl e0 => Gl (subE x e e0)
-      | loc_offset e1 e2 => loc_offset (sublE x e e1) (subE x e e2) 
-    end.
-  (* b[x/e]*)
-  Fixpoint subB x e b :=
-    match b with
-    | Bcomp op e1 e2 => Bcomp op (subE x e e1) (subE x e e2)
-    | Bbool op b1 b2 => Bbool op (subB x e b1) (subB x e b2)
-    | Bunary op b1 => Bunary op (subB x e b1)
-    end.
+(* Section Substitution. *)
+(*   (* from CSLsound.v *) *)
+(*   Fixpoint subE x e e0 :=  *)
+(*     match e0 with  *)
+(*       | Evar y => (if var_eq_dec x y then e else Evar y) *)
+(*       | Enum n => Enum n *)
+(*       | Eunop op b1 => Eunop op (subE x e b1) *)
+(*       | Ebinop op e1 e2 => Ebinop op (subE x e e1) (subE x e e2) *)
+(*     end. *)
+(*   Fixpoint sublE x e e0 :=  *)
+(*     match e0 with  *)
+(*       | Loff e1 e2 => Loff (subE x e e1) (subE x e e2)  *)
+(*     end. *)
 
-  Lemma subE_assign : forall (x : var) (e e' : exp) (s : stack),
-    edenot (subE x e e') s = edenot e' (var_upd s x (edenot e s)).
-  Proof.
-    intros; induction e'; simpl; eauto; unfold var_upd; 
-    repeat match goal with [ |- context[if ?X then _ else _]] => 
-                           destruct X
-           end; try congruence; eauto; f_equal; eauto;
-    rewrite IHe'1, IHe'2 in *; tauto.
-  Qed.
+(*   Lemma subE_assign : forall (x : var) (e e' : exp) (s : stack), *)
+(*       edenote (subE x e e') s = match edenote e s with *)
+(*                                 | Some v => edenote e' (var_upd s x v) *)
+(*                                 | None =>  *)
+(*   Proof. *)
+(*     intros; induction e'; simpl; eauto; unfold var_upd;  *)
+(*     repeat match goal with [ |- context[if ?X then _ else _]] =>  *)
+(*                            destruct X *)
+(*            end; try congruence; eauto; f_equal; eauto; *)
 
-  Lemma sublE_assign : forall (x : var) (e : exp) (e' : loc_exp) (s : stack),
-    ledenot (sublE x e e') s = ledenot e' (var_upd s x (edenot e s)).
-  Proof.
-    intros; induction e'; simpl; try destruct p; simpl; eauto; rewrite subE_assign; eauto.
-    rewrite IHe'; auto.
-  Qed.
+(*       rewrite IHe'1, IHe'2 in *; tauto. *)
+(*   Qed. *)
 
-  Lemma subB_assign : forall (x : var) (e : exp) (b : bexp) (s : stack),
-    bdenot (subB x e b) s = bdenot b (var_upd s x (edenot e s)).
-  Proof.
-    intros; induction b; simpl;
-    repeat match goal with [ |- context[if Z.eq_dec ?x ?y then _ else _]] => 
-                           destruct (Z.eq_dec x y) end;
-    repeat match goal with [ |- context[if Z_lt_dec ?x ?y then _ else _]] => 
-                           destruct (Z_lt_dec x y) end;
-    repeat rewrite subE_assign in *; congruence.
-  Qed.
-End Substitution.
+(*   Lemma sublE_assign : forall (x : var) (e : exp) (e' : loc_exp) (s : stack), *)
+(*     ledenot (sublE x e e') s = ledenot e' (var_upd s x (edenot e s)). *)
+(*   Proof. *)
+(*     intros; induction e'; simpl; try destruct p; simpl; eauto; rewrite subE_assign; eauto. *)
+(*     rewrite IHe'; auto. *)
+(*   Qed. *)
 
-Notation simple_heap := (PHeap.heap Z).
+(*   Lemma subB_assign : forall (x : var) (e : exp) (b : bexp) (s : stack), *)
+(*     bdenot (subB x e b) s = bdenot b (var_upd s x (edenot e s)). *)
+(*   Proof. *)
+(*     intros; induction b; simpl; *)
+(*     repeat match goal with [ |- context[if Z.eq_dec ?x ?y then _ else _]] =>  *)
+(*                            destruct (Z.eq_dec x y) end; *)
+(*     repeat match goal with [ |- context[if Z_lt_dec ?x ?y then _ else _]] =>  *)
+(*                            destruct (Z_lt_dec x y) end; *)
+(*     repeat rewrite subE_assign in *; congruence. *)
+(*   Qed. *)
+(* End Substitution. *)
+
+Notation simple_heap := (@PHeap.heap Z val).
 
 Section GlobalSemantics.
   Variable nblk : nat.
